fstar/new/Test.Encryption.fst
@@ -1,0 +1,76 @@
+module Test.Encryption
+
+open FStar.IO
+open FStar.All
+open Lib.ByteSequence
+open Test.Types
+open Test.Utils
+open TreeDEM
+open Crypto
+open Lib.Result
+open Tree
+
+module TreeMath = TreeMath
+
+val test_leaf_generation: #cs:ciphersuite -> ratchet_state cs -> encryption_leaf_generation_test -> ML (bool & ratchet_state cs)
+let test_leaf_generation #cs r_state test =
+  let (r_output, r_next_state) = extract_result (ratchet_next_key r_state) in
+  let key_ok = check_equal "key" string_to_string test.elgt_key (bytes_to_hex_string r_output.ro_key) in
+  let nonce_ok = check_equal "nonce" string_to_string test.elgt_nonce (bytes_to_hex_string r_output.ro_nonce) in
+  (key_ok && nonce_ok, r_next_state)
+
+val test_leaf_generations: #cs:ciphersuite -> ratchet_state cs -> list encryption_leaf_generation_test -> ML bool
+let rec test_leaf_generations #cs r_state tests =
+  match tests with
+  | [] -> true
+  | h::t ->
+    let (head_ok, r_next_state) = test_leaf_generation r_state h in
+    let tail_ok = test_leaf_generations r_next_state t in
+    head_ok && tail_ok
+
+val test_leaf: ciphersuite -> l:nat -> n:tree_size l -> i:leaf_index n -> bytes -> encryption_leaf_test -> ML bool
+let test_leaf cs l n i encryption_secret test =
+  let leaf_encryption_secret = extract_result (leaf_kdf n cs encryption_secret (TreeMath.root l) i) in
+  let i_as_node_index: TreeMath.node_index 0 = i+i in
+  let handshake_ratchet = extract_result (init_handshake_ratchet cs i_as_node_index leaf_encryption_secret) in
+  let application_ratchet = extract_result (init_application_ratchet cs i_as_node_index leaf_encryption_secret) in
+  let handshake_ok = test_leaf_generations handshake_ratchet test.handshake in
+  let application_ok = test_leaf_generations application_ratchet test.application in
+  handshake_ok && application_ok
+
+val test_leaves_aux: ciphersuite -> l:nat -> n:tree_size l -> bytes -> leaf_tests:list encryption_leaf_test -> i:nat{i + List.Tot.length leaf_tests <= n} -> ML bool
+let rec test_leaves_aux cs l n encryption_secret leaf_tests i =
+  match leaf_tests with
+  | [] -> true
+  | h::t ->
+    let head_ok = test_leaf cs l n i encryption_secret h in
+    let tail_ok = test_leaves_aux cs l n encryption_secret t (i+1) in
+    head_ok && tail_ok
+
+val test_leaves: ciphersuite -> l:nat -> n:tree_size l -> bytes -> leaf_tests:list encryption_leaf_test{List.Tot.length leaf_tests <= n} -> ML bool
+let test_leaves cs l n encryption_secret leaf_tests =
+  test_leaves_aux cs l n encryption_secret leaf_tests 0
+
+val test_encryption_one: encryption_test -> ML bool
+let test_encryption_one t =
+  match uint16_to_ciphersuite t.et_cipher_suite with
+  | Error s -> begin
+    IO.print_string ("Skipping one test because of missing ciphersuite: '" ^ s ^ "'\n");
+    true
+  end
+  | Success cs -> begin
+    let n_leaves = UInt32.v t.et_n_leaves in
+    let n_nodes = n_leaves + n_leaves - 1 in
+    let l = if n_nodes > 0 then (TreeMath.Internal.log2 n_nodes) + 1 else failwith "there cannot be 0 leaves!" in
+    let leaves_ok =
+      if List.Tot.length t.et_leaves <= n_leaves then
+        test_leaves cs l n_leaves (hex_string_to_bytes t.et_encryption_secret) t.et_leaves
+      else
+        failwith "list leaves is too big!"
+    in
+    leaves_ok
+  end
+
+val test_encryption: list encryption_test -> ML bool
+let test_encryption =
+  test_list "Encryption" test_encryption_one
